PLeaTTa/Proofs/PrologFindallAnswerResourceBridge.lean
@@ -80,7 +80,7 @@ theorem append_alts
         afterAlts _ =>
       AnswerOriginResourceAgrees alpha origin beforeResources afterResources
         (beforeAlts ++ suffix) (afterAlts ++ suffix))
-    (fun _ _ _ _ => True.intro)
+    (by intros; trivial)
     (by intros; trivial)
     (by intros; trivial)
     (fun leafScope bindings resources alts =>
